Complete typechecker
Removed check for constr valid because implied by wf
Removed strong positivity for now bc we don't have functions
Did mut, rest of function, indprop cases for typechecker
Gave incremental and full function and proved correctness

proofs/core/Typechecker.v
@@ -751,165 +751,117 @@ Section ContextCheck.
 
 Variable gamma: context.
 
-(*Here, we show that the context checks (some of them for now)
-  are decidable.
-  We need this for some proofs; namely for recursive functions, 
-  we need to be able to find the fs and ps to build our function*)
+(*Part 1: wf_funsym and wf_predsym*)
 
-(*Fixpoint check_valid_matches_tm (t: term) : bool :=
-  match t with
-  | Tfun f vs tms =>
-    all check_valid_matches_tm tms
-  | Tlet tm1 v tm2 =>
-    check_valid_matches_tm tm1 &&
-    check_valid_matches_tm tm2
-  | Tif f1 t1 t2 =>
-    check_valid_matches_fmla f1 &&
-    check_valid_matches_tm t1 &&
-    check_valid_matches_tm t2
-  | Tmatch t1 v ps =>
-    check_valid_matches_tm t1 &&
-    is_vty_adt gamma v &&
-    all (fun x => check_valid_matches_tm (snd x)) ps
-  | Teps f v =>
-    check_valid_matches_fmla f
-  | _ => true
-  end
-with check_valid_matches_fmla (f: formula) : bool :=
-  match f with
-  | Fpred p vs tms => all check_valid_matches_tm tms
-  | Fquant q v f => check_valid_matches_fmla f
-  | Feq v t1 t2 => check_valid_matches_tm t1 &&
-    check_valid_matches_tm t2
-  | Fbinop b f1 f2 => check_valid_matches_fmla f1 &&
-    check_valid_matches_fmla f2
-  | Fnot f => check_valid_matches_fmla f
-  | Flet t v f => check_valid_matches_tm t &&
-    check_valid_matches_fmla f
-  | Fif f1 f2 f3 =>
-    check_valid_matches_fmla f1 &&
-    check_valid_matches_fmla f2 &&
-    check_valid_matches_fmla f3
-  | Fmatch t v ps =>
-    check_valid_matches_tm t &&
-    is_vty_adt gamma v &&
-    all (fun x => check_valid_matches_fmla (snd x)) ps
-  | _ => true
-  end.*)
+Definition check_wf_funsym (f: funsym) : bool :=
+  all (fun t => typecheck_type gamma t &&
+    all (fun x => x \in (s_params f)) (type_vars t))
+  (f_ret f :: s_args f).
 
-(*We could assume stuff, but let's just plow through
-  this I guess*)
+Lemma check_wf_funsym_spec (f: funsym):
+  reflect (wf_funsym gamma f) (check_wf_funsym f).
+Proof.
+  rewrite /check_wf_funsym/wf_funsym.
+  apply all_Forall=> x Hinx.
+  apply andPP; first by apply typecheck_type_correct.
+  apply all_Forall=> v Hinv.
+  apply /inP.
+Qed.
+
+Definition check_wf_predsym (p: predsym) : bool :=
+  all (fun t => typecheck_type gamma t &&
+    all (fun x => x \in (s_params p)) (type_vars t))
+  (s_args p).
+
+Lemma check_wf_predsym_spec (p: predsym):
+  reflect (wf_predsym gamma p) (check_wf_predsym p).
+Proof.
+  rewrite /check_wf_predsym/wf_predsym.
+  apply all_Forall => x Hinx.
+  apply andPP; first by apply typecheck_type_correct.
+  apply all_Forall => v Hinv.
+  apply /inP.
+Qed.
+
+(*Part 2: definition check*)
+
+(*Checks for datatypes*)
+
+Section Datatype.
+
+Definition adt_valid_type_check (a: alg_datatype) : bool :=
+  match a with
+  | alg_def ts constrs =>
+    all (fun (c: funsym) => ((s_params c) == (ts_args ts)) &&
+      ((f_ret c) == vty_cons ts (map vty_var (ts_args ts))))
+      (ne_list_to_list constrs)
+  end.
+
+Lemma adt_valid_type_check_spec (a: alg_datatype) :
+  reflect (adt_valid_type a) (adt_valid_type_check a).
+Proof.
+  rewrite /adt_valid_type /adt_valid_type_check.
+  case: a => [ts constrs].
+  apply all_Forall => x Hinx.
+  by apply andPP; apply eqP.
+Qed.
+
+Definition valid_mut_rec_check (m: mut_adt) : bool :=
+  all (fun a => ((m_params m) == (ts_args (adt_name a))) &&
+    all (fun (f: funsym) => m_params m == s_params f)
+      (adt_constr_list a))
+  (typs m).
+
+Lemma valid_mut_rec_check_spec m :
+  reflect (valid_mut_rec m) (valid_mut_rec_check m).
+Proof.
+  rewrite /valid_mut_rec /valid_mut_rec_check.
+  apply forallb_ForallP => x Hinx.
+  apply andPP; first by apply eqP.
+  apply all_Forall => y Hiny.
+  by apply eqP.
+Qed.
+
+(*The whole check is easy, since the most difficult check
+  (inhab) is a boolean already
+  TODO: strictly positive or something?*)
+Definition mut_valid_check (m: mut_adt) : bool :=
+  all (adt_valid_type_check) (typs m) &&
+  all (adt_inhab gamma) (typs m) &&
+  valid_mut_rec_check m &&
+  uniform m.
+
+Lemma mut_valid_check_spec (m: mut_adt) :
+  reflect (mut_valid gamma m) (mut_valid_check m).
+Proof.
+  rewrite /mut_valid/mut_valid_check.
+  rewrite - !andbA.
+  repeat (apply andPP).
+  - apply forallb_ForallP => x Hinx. 
+    by apply adt_valid_type_check_spec.
+  - apply forallb_ForallP=> y Hiny.
+    by apply idP.
+  - by apply valid_mut_rec_check_spec.
+  - by apply idP.
+Qed.
+
+End Datatype.
+
+(*Recursive functions *)
+
+Section RecFun.
+
+(*This is much harder, since we need to find the decreasing arguments
+  (and prove that the decreasing check itself is decidable).
+  We also need this typechecking to define the full recursive
+  function implementation in RecFun2.v*)
+
 Definition pattern_eqMixin := EqMixin pattern_eqb_spec.
 Canonical pattern_eqType := EqType pattern pattern_eqMixin.
 Definition term_eqMixin := EqMixin term_eqb_spec.
 Canonical term_eqType := EqType term term_eqMixin.
 Definition formula_eqMixin := EqMixin formula_eqb_spec.
 Canonical formula_eqType := EqType formula formula_eqMixin.
-(*
-Lemma iter_and_Forall {A: Type} {P: A -> Prop} {l: list A}:
-  Forall P l <-> iter_and (List.map P l).
-Proof.
-  elim: l=>//= h t IH/=.
-  split =>[Hall | [Hh Ht]].
-  - split.
-    + exact (Forall_inv Hall).
-    + rewrite -IH. exact (Forall_inv_tail Hall).
-  - constructor=>//. by apply IH.
-Qed.
-
-Lemma check_valid_matches_spec (t: term) (f: formula):
-  reflect (valid_matches_tm gamma t) (check_valid_matches_tm t) *
-  reflect (valid_matches_fmla gamma f) (check_valid_matches_fmla f).
-Proof.
-  revert t f; apply term_formula_rect =>//=;
-  (try by (intros; apply ReflectT));
-  try by (intros; apply andPP).
-  (*Only 3 nontrivial cases for each: fun/pred, if (basically trivial),
-  and match*)
-  - move=> f1 tys tms Hall.
-    eapply equivP. 2: apply iter_and_Forall.
-    apply all_Forall. 
-    move: Hall; elim: tms => [//=| thd ttl IH /= Hall x].
-    rewrite in_cons. (*Can't destruct on or*)
-    case: (x == thd) /eqP => [Hxh _ | Hneq]/=; subst.
-    + exact (ForallT_hd _ _ _ Hall).
-    + apply IH. exact (ForallT_tl _ _ _ Hall).
-  - move=> f t1 t2 IH1 IH2 IH3.
-    rewrite -andbA.
-    repeat apply andPP=>//.
-  - move=> tm v ps IH1 Hall. cbn.
-    rewrite -andbA.
-    repeat apply andPP=>//.
-    + apply is_vty_adt_weak.
-    + eapply equivP. 2: apply iter_and_Forall.
-      apply all_Forall.
-      move: Hall.
-      elim: ps => //= [[p1 t1]] tl IH Hall x.
-      rewrite in_cons.
-      case: (x == (p1, t1)) /eqP => /=[Hxp1 _ | Hneq ]; subst=>/=.
-      * exact (ForallT_hd _ _ _ Hall).
-      * apply IH. exact (ForallT_tl _ _ _ Hall).
-  - move=> p tys tms Hall.
-    eapply equivP. 2: apply iter_and_Forall.
-    apply all_Forall. 
-    move: Hall; elim: tms => [//=| thd ttl IH /= Hall x].
-    rewrite in_cons. (*Can't destruct on or*)
-    case: (x == thd) /eqP => [Hxh _ | Hneq]/=; subst.
-    + exact (ForallT_hd _ _ _ Hall).
-    + apply IH. exact (ForallT_tl _ _ _ Hall).
-  - move=> f1 f2 f3 IH1 IH2 IH3.
-    rewrite -andbA.
-    repeat apply andPP=>//.
-  - move=> tm v ps IH1 Hall. cbn.
-    rewrite -andbA.
-    repeat apply andPP=>//.
-    + apply is_vty_adt_weak.
-    + eapply equivP. 2: apply iter_and_Forall.
-      apply all_Forall.
-      move: Hall.
-      elim: ps => //= [[p1 t1]] tl IH Hall x.
-      rewrite in_cons.
-      case: (x == (p1, t1)) /eqP => /=[Hxp1 _ | Hneq ]; subst=>/=.
-      * exact (ForallT_hd _ _ _ Hall).
-      * apply IH. exact (ForallT_tl _ _ _ Hall).
-Qed.
-
-Definition check_valid_matches_tm_spec t := 
-  fst (check_valid_matches_spec t Ftrue).
-Definition check_valid_matches_fmla_spec f := 
-  snd (check_valid_matches_spec tm_d f).*)
-
-(*Well-typed terms*)
-(*
-Definition check_well_typed_tm (t: term) (ty: vty) : bool :=
-  (typecheck_term sigma t == Some ty) &&
-  check_valid_matches_tm t.
-
-Definition check_well_typed_fmla (f: formula) : bool :=
-  (typecheck_formula sigma f) &&
-  check_valid_matches_fmla f.
-
-Lemma check_well_typed_tm_spec (t: term) (ty: vty):
-  reflect (well_typed_term sigma gamma t ty) (check_well_typed_tm t ty).
-Proof.
-  apply andPP.
-  apply typecheck_term_correct.
-  apply check_valid_matches_tm_spec.
-Qed.
-
-Lemma check_well_typed_fmla_spec (f: formula):
-  reflect (well_typed_formula sigma gamma f) (check_well_typed_fmla f).
-Proof.
-  apply andPP.
-  apply typecheck_formula_correct.
-  apply check_valid_matches_fmla_spec.
-Qed.*)
-
-(*TODO: [adt_valid_type], inhabited types, strict positivity
-  for types (TODO: add uniformity)*)
-
-(*Checks for recursive functions*)
-
 
 Definition check_funpred_def_valid_type (fd: funpred_def) : bool :=
   match fd with
@@ -2274,6 +2226,7 @@ Proof.
   - by rewrite -size_split_funpred_defs_fst.
 Qed.
 
+Section WFCtx.
 Variable gamma_wf: wf_context gamma.
 
 
@@ -2498,6 +2451,525 @@ Proof.
     by apply (find_funpred_def_term_none l Hin Hfind m params vs il).
 Qed.
 
+End WFCtx.
+
+(*The other half: funpred_def_valid_type*)
+
+Definition funpred_def_valid_type_check (fd: funpred_def): bool :=
+  match fd with
+  | fun_def f vars t =>
+    (typecheck_term gamma t == Some (f_ret f)) &&
+    (sublistb (tm_fv t) vars) &&
+    (sublistb (tm_type_vars t) (s_params f)) &&
+    (uniq (map fst vars)) &&
+    (map snd vars == (s_args f))
+  | pred_def p vars f =>
+    (typecheck_formula gamma f) &&
+    (sublistb (fmla_fv f) vars) &&
+    (sublistb (fmla_type_vars f) (s_params p)) &&
+    (uniq (map fst vars)) &&
+    ((map snd vars) == (s_args p))
+  end.
+
+Lemma funpred_def_valid_type_check_spec (fd: funpred_def) :
+  reflect (funpred_def_valid_type gamma fd) 
+    (funpred_def_valid_type_check fd).
+Proof.
+  rewrite /funpred_def_valid_type/funpred_def_valid_type_check.
+  case: fd => [f vars t | p vars f];
+  rewrite -!andbA; repeat (apply andPP);
+  try (apply sublistbP);
+  try (apply uniqP);
+  try (apply eqP).
+  - apply typecheck_term_correct.
+  - apply typecheck_formula_correct.
+Qed.
+
+(*And now the full check for functions*)
+Definition funpred_valid_check (l: list funpred_def) : bool :=
+  all (funpred_def_valid_type_check) l &&
+  (isSome (find_funpred_def_term l)).
+
+Lemma funpred_valid_check_spec (l: list funpred_def) :
+  wf_context gamma ->
+  l \in mutfuns_of_context gamma ->
+  reflect (funpred_valid gamma l) (funpred_valid_check l).
+Proof.
+  move=> Hwf l_in.
+  rewrite /funpred_valid/funpred_valid_check.
+  apply andPP.
+  - apply all_Forall=> x Hinx.
+    apply funpred_def_valid_type_check_spec.
+  - (*This one is a bit tougher*)
+    rewrite /funpred_def_term_exists.
+    case Hfind: (find_funpred_def_term l) => [[[[m params] vs] il] |]/=.
+    + apply ReflectT.
+      exists m. exists params. exists vs. exists il.
+      by apply find_funpred_def_term_some.
+    + apply ReflectF.
+      move=> [m [params [vs [il Hdef]]]].
+      by apply (find_funpred_def_term_none Hwf l l_in Hfind m params vs il).
+Qed.
+
+End RecFun.
+
+(*Inductive predicates*)
+Print valid_def.
+
+
+Print indprop_valid.
+
+Print indprop_valid_type.
+
+Print valid_ind_form.
+
+(*[valid_ind_form]*)
+Fixpoint valid_ind_form_check (p: predsym) (f: formula) : bool :=
+  match f with
+  | Fpred p' tys tms =>
+    (p == p') && (tys == map vty_var (s_params p)) &&
+    (length (s_args p) == length tms)
+  | Fbinop Timplies f1 f2 =>
+    valid_ind_form_check p f2
+  | Fquant Tforall x f =>
+    valid_ind_form_check p f
+  | Flet t x f =>
+    valid_ind_form_check p f
+  | _ => false
+  end.
+
+Lemma valid_ind_form_check_spec (p: predsym) (f: formula):
+  reflect (valid_ind_form p f) (valid_ind_form_check p f).
+Proof.
+  move: f.
+  apply (formula_rect (fun _ => True) (fun f => 
+  reflect (valid_ind_form p f) (valid_ind_form_check p f) ))=>//=;
+  intros; try by reflF.
+  - case: (p == p0) /eqP=>/= Hpp0; last by reflF.
+    rewrite -Hpp0.
+    case: (tys == [seq vty_var i | i <- s_params p]) /eqP => /= Htys;
+    last by reflF.
+    case: (length (s_args p) == length tms) /eqP => /= Hlens;
+    last by reflF.
+    by reflT.
+  - case: q; last by reflF. 
+    case: H => Hval; last by reflF. by reflT.
+  - case: b; try by reflF.
+    case: H0 => Hval; last by reflF. by reflT.
+  - case: H0 => Hval; last by reflF. by reflT.
+Qed.
+
+Print indprop_valid_type.
+
+Definition indprop_valid_type_check (i: indpred_def) : bool :=
+  match i with
+  | ind_def p lf =>
+    all (fun (f: formula) =>
+      typecheck_formula gamma f &&
+      closed_formula f &&
+      valid_ind_form_check p f &&
+      sublistb (fmla_type_vars f) (s_params p)
+      ) (map snd lf)
+  end.
+
+Lemma indprop_valid_type_check_spec (i: indpred_def) :
+  reflect (indprop_valid_type gamma i) (indprop_valid_type_check i).
+Proof.
+  rewrite /indprop_valid_type/indprop_valid_type_check.
+  case: i => [p lf].
+  apply all_Forall=> x Hinx.
+  rewrite - !andbA. repeat (apply andPP).
+  - apply typecheck_formula_correct.
+  - apply idP.
+  - apply valid_ind_form_check_spec.
+  - apply sublistbP.
+Qed.
+
+(*Now [indpred_positive]*)
+Print indpred_positive.
+
+Print ind_positive.
+
+Print ind_strictly_positive.
+
+Fixpoint ind_strictly_positive_check (ps: seq predsym) (f: formula)
+  {struct f} : bool :=
+  (all (fun p => ~~ predsym_in_fmla p f) ps) ||
+  match f with
+  | Fpred p vs ts =>
+    (p \in ps) &&
+    all (fun t => all (fun x => ~~ predsym_in_tm x t) ps ) ts
+  | Fbinop Timplies f1 f2 =>
+    ind_strictly_positive_check ps f2 &&
+    all (fun p => ~~ predsym_in_fmla p f1) ps
+  | Fquant q x f =>
+    ind_strictly_positive_check ps f
+  | Fbinop Tand f1 f2 =>
+    ind_strictly_positive_check ps f1 &&
+    ind_strictly_positive_check ps f2
+  | Fbinop Tor f1 f2 =>
+    ind_strictly_positive_check ps f1 &&
+    ind_strictly_positive_check ps f2
+  | Flet t x f =>
+    all (fun p => ~~ predsym_in_tm p t) ps &&
+    ind_strictly_positive_check ps f
+  | Fif f1 f2 f3 =>
+    all (fun p => ~~ predsym_in_fmla p f1) ps &&
+    ind_strictly_positive_check ps f2 &&
+    ind_strictly_positive_check ps f3
+  | Fmatch t ty pats =>
+    all (fun p => ~~ predsym_in_tm p t) ps &&
+    (*to satisfy positivity checker*)
+    all id (map (fun x => ind_strictly_positive_check ps (snd x)) pats)
+  | _ => false
+  end.
+
+(*Want to handle notin case at beginning*)
+Ltac not_in_pos_case ps f :=
+  let Hallin := fresh "Hallin" in
+  case: (all (fun p => ~~ predsym_in_fmla p f) ps) 
+    /(all_Forall _ _ _ (fun x Hin => idP))=>/= Hallin;
+    rewrite -> Forall_forall in Hallin; first by
+      apply ReflectT; constructor.
+
+Lemma all_id_map {A: Type} {p: pred A} {s: seq A}:
+  all id (map p s) = all p s.
+Proof.
+  by elim: s => [// | h t /= ->].
+Qed.
+  
+
+Lemma ind_strictly_positive_check_spec (ps: seq predsym) (f: formula) :
+  reflect (ind_strictly_positive ps f) (ind_strictly_positive_check ps f).
+Proof.
+  move: f.
+  apply (formula_rect (fun _ => true) (fun f => 
+  reflect (ind_strictly_positive ps f) (ind_strictly_positive_check ps f)))=>//=;
+  intros.
+  - not_in_pos_case ps (Fpred p tys tms).
+    case:(p \in ps) /inP => Hinp/=; last by reflF.
+    case: (all (fun t : term => all (fun x : predsym => ~~ predsym_in_tm x t) ps) tms)
+      /(all_Forall (fun t => Forall (fun x => ~~ predsym_in_tm x t) ps)).
+    + move=>x Hinx. apply all_Forall=> y Hiny. apply idP.
+    + move=> Hall2. apply ReflectT. apply ISP_pred=>//.
+      move=> x t Hint Hinx.
+      move: Hall2.
+      rewrite -> Forall_forall => /(_ _ Hint).
+      by rewrite -> Forall_forall => /(_ _ Hinx).
+    + move=> Hnotall. apply ReflectF. move=> C; inversion C; subst=>//.
+      apply Hnotall.
+      rewrite Forall_forall => t Hint.
+      rewrite Forall_forall=> x. by apply H4.
+  - not_in_pos_case ps (Fquant q v f).
+    case: H => Hpos. by reflT. by reflF.
+  - not_in_pos_case ps (Feq v t1 t2).
+    by reflF.
+  - not_in_pos_case ps (Fbinop b f1 f2).
+    case: b; try by reflF.
+    + case: H => Hpos1; last by reflF.
+      case: H0 => Hpos2; last by reflF.
+      by reflT.
+    + case: H => Hpos1; last by reflF.
+      case: H0 => Hpos2; last by reflF.
+      by reflT.
+    + case: H0 => Hpos; last by reflF.
+      case: (all (fun p : predsym => ~~ predsym_in_fmla p f1) ps) 
+        /(all_Forall _ _ _ (fun _ _ => idP)) => Hall;
+      rewrite -> Forall_forall in Hall;
+      last by reflF.
+      by reflT.
+  - not_in_pos_case ps (Fnot f). by reflF.
+  - not_in_pos_case ps Ftrue. by reflF.
+  - not_in_pos_case ps Ffalse. by reflF.
+  - not_in_pos_case ps (Flet tm v f).
+    case: (all (fun p : predsym => ~~ predsym_in_tm p tm) ps)
+    /(all_Forall _ _ _ (fun _ _ => idP)) => Hall;
+    rewrite -> Forall_forall in Hall;
+    last by reflF.
+    case: H0 => Hpos; last by reflF.
+    by reflT.
+  - not_in_pos_case ps (Fif f1 f2 f3).
+    case: (all (fun p : predsym => ~~ predsym_in_fmla p f1) ps) 
+    /(all_Forall _ _ _ (fun _ _ => idP)) => Hall;
+    rewrite -> Forall_forall in Hall;
+    last by reflF.
+    case: H0=> Hpos1; last by reflF.
+    case: H1=> Hpos2; last by reflF.
+    by reflT.
+  - not_in_pos_case ps (Fmatch tm v ps0).
+    case: (all (fun p : predsym => ~~ predsym_in_tm p tm) ps)
+    /(all_Forall _ _ _ (fun _ _ => idP)) => Hall;
+    rewrite -> Forall_forall in Hall;
+    last by reflF.
+    have Hrefl: reflect (forall f : formula,
+    In f (List.map snd ps0) -> ind_strictly_positive ps f)
+    (all id [seq ind_strictly_positive_check ps x.2 | x <- ps0]). {
+      eapply equivP. 2: apply Forall_forall.
+      rewrite all_id_map.
+      eapply equivP. 2: symmetry; apply Forall_map.
+      apply all_Forall.
+      move=> x /inP Hinx.
+      apply (ForallT_In _ formula_eq_dec _ H0).
+      rewrite in_map_iff. by exists x.
+    }
+    case: Hrefl => Hallpos; last by reflF.
+    by reflT.
+Qed.
+
+Fixpoint ind_positive_check (ps: seq predsym) (f: formula) : bool :=
+  match f with
+  | Fpred p vs ts =>
+    (p \in ps) &&
+    all (fun t => all (fun x => ~~ predsym_in_tm x t) ps ) ts
+  | Fquant Tforall x f =>
+    ind_positive_check ps f
+  | Flet t x f =>
+    all (fun p => ~~ predsym_in_tm p t) ps &&
+    ind_positive_check ps f
+  | Fbinop Timplies f1 f2 =>
+    ind_strictly_positive_check ps f1 &&
+    ind_positive_check ps f2
+  | _ => false
+  end.
+
+(*Some duplication with previous proof*)
+Lemma ind_positive_check_spec (ps: seq predsym) (f: formula) : 
+  reflect (ind_positive ps f) (ind_positive_check ps f).
+Proof.
+  apply (formula_rect (fun _ => True) (fun f =>
+  reflect (ind_positive ps f) (ind_positive_check ps f)))=>//=;
+  intros; try by reflF.
+  - case:(p \in ps) /inP => Hinp/=; last by reflF.
+    case: (all (fun t : term => all (fun x : predsym => ~~ predsym_in_tm x t) ps) tms)
+      /(all_Forall (fun t => Forall (fun x => ~~ predsym_in_tm x t) ps)).
+    + move=>x Hinx. apply all_Forall=> y Hiny. apply idP.
+    + move=> Hall2. apply ReflectT. apply IP_pred=>//.
+      move=> x t Hint Hinx.
+      move: Hall2.
+      rewrite -> Forall_forall => /(_ _ Hint).
+      by rewrite -> Forall_forall => /(_ _ Hinx).
+    + move=> Hnotall. apply ReflectF. move=> C; inversion C; subst=>//.
+      apply Hnotall.
+      rewrite Forall_forall => t Hint.
+      rewrite Forall_forall=> x. by apply H4.
+  - case: q; last by reflF.
+    case: H=> Hpos; last by reflF.
+    by reflT.
+  - case: b; try by reflF.
+    case: (ind_strictly_positive_check_spec ps f1) => Hpos1;
+    last by reflF.
+    case: H0 => Hpos2; last by reflF.
+    by reflT.
+  - case: (all (fun p : predsym => ~~ predsym_in_tm p tm) ps)
+    /(all_Forall _ _ _ (fun _ _ => idP)) => Hall;
+    rewrite -> Forall_forall in Hall;
+    last by reflF.
+    case: H0 => Hpos; last by reflF.
+    by reflT.
+Qed.
+
+Definition indpred_positive_check (l: seq indpred_def) : bool :=
+  let ps :=
+    map (fun i => match i with | ind_def p _ => p end) l in
+  let fs :=
+    concat (map (fun i => match i with | ind_def _ fs => map snd fs end) l)
+  in
+  all (ind_positive_check ps) fs.
+
+Lemma indpred_positive_check_spec (l: seq indpred_def) :
+  reflect (indpred_positive l) (indpred_positive_check l).
+Proof.
+  rewrite /indpred_positive/indpred_positive_check.
+  apply all_Forall.
+  move=> x Hinx.
+  apply ind_positive_check_spec.
+Qed.
+
+Print Forall_eq.
+(*[indpred_params_same]*)
+
+(*A faster check than using "all" at each iteration (from the
+  definition)*)
+
+Definition all_eq {A: Type} {B: eqType} (f: A -> B) (l: seq A) : bool :=
+  match l with
+  | nil => true
+  | h :: t => all (fun x => f x == f h) t
+  end.
+
+Lemma all_eq_spec {A: Type} {B: eqType}(f: A -> B) (l: seq A)  :
+  reflect (forall x y, In x l -> In y l -> f x = f y)
+    (all_eq f l).
+Proof.
+  rewrite /all_eq.
+  case: l=>[| h t]; first by apply ReflectT.
+  eapply equivP.
+  apply (forallb_ForallP (fun y => f y = f h));
+  first by move=> x Hinx; apply eqP.
+  rewrite -> Forall_forall. split=> Hallin x.
+  - move=> y [Hxh | Hxt] [Hyh | Hyt]; subst=>//;
+    try (by apply Hallin);
+    try (symmetry; by apply Hallin).
+    rewrite Hallin //. symmetry.
+    by rewrite Hallin.
+  - move=> Hinx. by apply Hallin=>/=; auto.
+Qed.
+
+Lemma all_eq_Forall_eq {A: Type} {B: eqType} (f: A -> B) (l: seq A):
+  reflect (Forall_eq f l) (all_eq f l).
+Proof.
+  apply iff_reflect.
+  rewrite -(reflect_iff _ _ (all_eq_spec f l)).
+  by apply Forall_eq_iff.
+Qed.
+
+Definition indpred_params_same_check (l: seq indpred_def) : bool :=
+  all_eq (fun i => match i with | ind_def p _ => s_params p end) l.
+
+Lemma indpred_params_same_check_spec (l: seq indpred_def) :
+  reflect (indpred_params_same l) (indpred_params_same_check l).
+Proof.
+  rewrite /indpred_params_same/indpred_params_same_check.
+  apply all_eq_Forall_eq.
+Qed.
+
+(*Now, full indprop def*)
+Definition indprop_valid_check (il: seq indpred_def) : bool :=
+  all indprop_valid_type_check il &&
+  indpred_positive_check il &&
+  indpred_params_same_check il &&
+  indpreds_uniform il.
+
+Lemma indprop_valid_check_spec (il: seq indpred_def) :
+  reflect (indprop_valid gamma il) (indprop_valid_check il).
+Proof.
+  rewrite /indprop_valid/indprop_valid_check.
+  rewrite -!andbA.
+  repeat (apply andPP).
+  - apply forallb_ForallP. move=> x Hinx.
+    apply indprop_valid_type_check_spec.
+  - apply indpred_positive_check_spec.
+  - apply indpred_params_same_check_spec.
+  - apply idP.
+Qed.
+
+(*And now, we can check an entire definition*)
+
+Definition valid_def_check (d: def) : bool :=
+  match d with
+  | datatype_def m => mut_valid_check m
+  | recursive_def fs => funpred_valid_check fs
+  | inductive_def l => indprop_valid_check l
+  | _ => true
+  end.
+
+Lemma valid_def_check_spec (d: def) :
+  wf_context gamma ->
+  In d gamma ->
+  reflect (valid_def gamma d) (valid_def_check d).
+Proof.
+  move=> Hwf.
+  rewrite /valid_def/valid_def_check.
+  case: d; try by (move=> _ _; apply ReflectT).
+  - move=> m _. apply mut_valid_check_spec.
+  - move=> l l_in. apply funpred_valid_check_spec=>//.
+    apply /inP.
+    by apply in_mutfuns.
+  - move=> l _. apply indprop_valid_check_spec.
+Qed.
+
 End ContextCheck.
+
+(*Now we show that we can incrementally check the context,
+  since we don't want to have to check it each time*)
+
+Definition check_context_cons (d: def) (gamma: context) : bool :=
+  let funs := funsyms_of_def d in
+  let preds := predsyms_of_def d in
+  let tys := typesyms_of_def d in
+  all (check_wf_funsym (d :: gamma)) funs &&
+  all (check_wf_predsym (d :: gamma)) preds &&
+  all (fun f => f \notin (sig_f gamma)) funs &&
+  all (fun p => p \notin (sig_p gamma)) preds &&
+  all (fun t => t \notin (sig_t gamma)) tys &&
+  uniq funs &&
+  uniq preds &&
+  uniq tys &&
+  nonempty_def d &&
+  valid_def_check (d :: gamma) d.
+
+(*If we start with a valid context, this check means that
+  our additional context is still valid*)
+Theorem check_context_cons_correct (d: def) (gamma: context) :
+  valid_context gamma ->
+  reflect (valid_context (d :: gamma)) (check_context_cons d gamma).
+Proof.
+  move=> Hval.
+  rewrite /check_context_cons.
+  (*First, wf_funsym and predsym*)
+  case: (all (check_wf_funsym (d :: gamma)) (funsyms_of_def d))
+    /(all_Forall (fun f => wf_funsym (d :: gamma) f)); 
+  last by move=> Hall; reflF.
+    by move=> x Hinx; apply check_wf_funsym_spec.
+  move=> Hfunswf.
+
+  case: (all (check_wf_predsym (d :: gamma)) (predsyms_of_def d))
+    /(all_Forall (fun p => wf_predsym (d :: gamma) p));
+  last by move=> Hall; reflF.
+    by move=> x Hinx; apply check_wf_predsym_spec.
+  move=> Hpredswf.
+
+  (*Now, sig_t checks*)
+  case: (all (fun f => f \notin sig_f gamma) (funsyms_of_def d))
+    /(all_Forall (fun f => ~ In f (sig_f gamma)));
+  last by move=> Hall; reflF.
+    by move=> x Hinx; apply negPP, inP.
+  move=> Hsigf.
+
+  case: (all (fun p => p \notin sig_p gamma) (predsyms_of_def d))
+    /(all_Forall (fun p => ~ In p (sig_p gamma)));
+  last by move=> Hall; reflF.
+    by move=> x Hinx; apply negPP, inP.
+  move=> Hsigp.
+
+  case: (all (fun t => t \notin sig_t gamma) (typesyms_of_def d))
+    /(all_Forall (fun t => ~ In t (sig_t gamma)));
+  last by move=> Hall; reflF.
+    by move=> x Hinx; apply negPP, inP.
+  move=> Hsigt.
+
+  (*Now NoDups checks for new definitions*)
+  case: (uniq (funsyms_of_def d)) /uniqP => Hnodupf; last by reflF.
+  case: (uniq (predsyms_of_def d)) /uniqP => Hnodupp; last by reflF.
+  case: (uniq (typesyms_of_def d)) /uniqP => Hnodupt; last by reflF.
+  case Hemp: (nonempty_def d); last 
+    by (apply ReflectF => C; inversion C; subst; rewrite Hemp in H10).
+  (*At this point, wf_context holds, so we can use the
+    def check lemma (the recfun case needs a wf_context)*)
+  have Hwf: wf_context (d :: gamma). {
+    apply valid_context_wf in Hval. by constructor.
+  }
+  case: (valid_def_check_spec (d :: gamma) d Hwf ltac:(simpl; auto))
+  => Hvald; last by reflF.
+  by reflT.
+Qed.
+
+(*A corollary: we can typecheck an entire context*)
+Fixpoint check_context (gamma: context) : bool :=
+  match gamma with
+  | nil => true
+  | d :: g => check_context g && check_context_cons d g
+  end.
+
+Theorem check_context_correct (gamma: context) :
+  reflect (valid_context gamma) (check_context gamma).
+Proof.
+  elim: gamma => [| d g /= IH].
+  - by reflT.
+  - case: IH => g_val; last by reflF.
+    case: (check_context_cons_correct d g g_val) => Hval;
+      last by apply ReflectF.
+    by apply ReflectT.
+Qed.
 
 End Typechecker.
